Split apart files, building up atomic library, added work on explode and similarity

src/cnf/cnf.lean
@@ -1,151 +1,111 @@
 /-
+This file contains the definitions of and basic operations on variables, literals,
+clauses, and conjunctive normal form.
 
-  This file contains the definitions of and basic operations on variables, literals,
-  clauses, and conjunctive normal form.
-
-  Authors: Cayden Codel, Jeremy Avigad, Marijn Heule
-  Carnegie Mellon University
-
+Authors: Cayden Codel, Jeremy Avigad, Marijn Heule
+Carnegie Mellon University
 -/
+
+-- TODO: by_cases can often replace classical.em (a = b), etc.
+
+import basic
+import cnf.literal
+import cnf.clause
 
 import data.list.basic
+import data.list.nodup
+import data.list.perm
 import init.data.nat
-
-/- 
-  All propositional formulas are comprised of Boolean variables.
-  Here, we represent variables as natural numbers, which may then be evaluated
-  with an appropriate assignment of boolean values to those variables.
-
-  Literals are positive and negative instances of those variables.
--/
-
-inductive literal : Type
-  | Pos : nat → literal
-  | Neg : nat → literal
-
-/- Assignments give boolean values to the variables -/
-def assignment := nat → bool
-
-namespace literal
-
-/- Negated literals receive the opposite boolean value as the variable -/
-def eval (α : assignment) : literal → bool
-  | (Pos n) := α n
-  | (Neg n) := bnot (α n)
-
-/- Extracts the natural number boolean variable of the literal -/
-def var : literal → nat
-  | (Pos n) := n
-  | (Neg n) := n
-
-def flip : literal → literal
-  | (Pos n) := Neg n
-  | (Neg n) := Pos n
-
-def set_pos : literal → literal
-  | (Pos n) := Pos n
-  | (Neg n) := Pos n
-
-def set_neg : literal → literal
-  | (Pos n) := Neg n
-  | (Neg n) := Neg n
-
-def is_pos : literal → bool
-  | (Pos _) := tt
-  | (Neg _) := ff
-
-def is_neg : literal → bool
-  | (Pos _) := ff
-  | (Neg _) := tt
-
-end literal
-
-/- (Disjunctive) clauses are lists of literals joined by logical ORs -/
-def clause := list literal
-
-namespace clause
-
---def length (c : clause) : nat := c.length
-
-/- The clause represents a disjunction, so we evaluate literals until tt is found -/
-def eval (α : assignment) (c : clause) : bool :=
-  c.foldr (λ l, λ b, b ∨ l.eval α) ff
-
-/- Counts the number of literals that evaluate to true in the clause, under some assignment -/
-def count_tt (α : assignment) (c : clause) : nat :=
-  list.length $ c.filter (λ l, l.eval α = tt)
-
-/- Counts the number of literals that evaluate to false in the clause, under some assignment -/
-def count_ff (α : assignment) (c : clause) : nat :=
-  list.length $ c.filter (λ l, l.eval α = ff)
-
-/- Counts the number of positive literals in the clause -/
-/- TODO why can't I use a match statement? Requires decidable_pred... -/
-def count_pos (c : clause) : nat :=
-  --list.length $ c.filter (λ l, match l with | (literal.Pos _) := true | _ := false end)
-  list.length $ c.filter (λ l, literal.is_pos l = tt)
-
-/- Counts the number of negative literals in the clause -/
-def count_neg (c : clause) : nat :=
-  list.length $ c.filter (λ l, literal.is_neg l = tt)
-
-/- Some useful statements for proofs of clauses -/
-lemma empty_eval_ff (α : assignment) (c : clause) : c.length = 0 → eval α c = ff :=
-begin
-  intro h,
-  rw list.length_eq_zero at h,
-  rw h,
-  unfold eval,
-  simp,
-end
-
-lemma single_eval_lit [inhabited literal] (α : assignment) (c : clause) : c.length = 1 → eval α c = c.head.eval α :=
-begin
-  intro h,
-  rw list.length_eq_one at h,
-  cases h with a ha,
-  unfold eval,
-  simp [ha],
-end
-
-end clause
+import data.nat.basic
 
 /- Conjunctive normal form is a list of clauses joined by logical ANDs -/
 def cnf := list clause
 
 namespace cnf
 
+open literal
+open clause
+open list
+
+/- Instance properties -/
+instance : inhabited cnf := ⟨[default clause]⟩
+
+instance : has_mem clause cnf := ⟨list.mem⟩
+
+instance : has_emptyc cnf := ⟨list.nil⟩
+
+instance : has_union cnf := ⟨list.union⟩
+
+instance : has_inter cnf := ⟨list.inter⟩
+
+instance : has_singleton clause cnf := ⟨λ c, [c]⟩ 
+
+instance : has_insert clause cnf := ⟨list.insert⟩
+
+instance : has_append cnf := ⟨list.append⟩
+
+/-! # sim_erase -/
+-- If we only care about evaluations, we can weaken the erase operation to removing similar clauses only
+-- See clause.eval_sim for motivation
+
+def sim_erase : cnf → clause → cnf
+| []          c := []
+| (cl :: cls) c := if cl ~ c then cls else cl :: sim_erase cls c
+
+-- Technically, sim_erase "inherits" a lot of functionality from erase, as it is weaker
+-- We reproduce only a few results here
+@[simp] theorem sim_erase_nil {c : clause} : sim_erase [] c = [] := rfl
+
+@[simp] theorem sim_erase_cons_head {c₁ c₂ : clause} {f : cnf} (h : c₁ ~ c₂) : sim_erase (c₁ :: f) c₂ = f :=
+by simp [sim_erase, h]
+
+theorem sim_erase_cons_tail {c₁ c₂ : clause} {f : cnf} (h : ¬(c₁ ~ c₂)) : sim_erase (c₁ :: f) c₂ = c₁ :: (sim_erase f c₂) :=
+by simp [sim_erase, h]
+
+theorem sim_erase_of_not_sim {c : clause} {f : cnf} (h : ∀ cl ∈ f, ¬(cl ~ c)) : sim_erase f c = f := by sorry
+/-
+by { induction f with cl cls ih, { exact sim_erase_nil },
+  unfold sim_erase, have : ¬ cl ~ c, from h cl (mem_cons_self cl cls), simp [this], }
+  -/
+
+/-! ### Eval -/
+
 /- The clauses of the CNF are joined by conjunctions, so all must evaluate to true -/
 def eval (α : assignment) (f : cnf) : bool :=
-  f.foldr (λ c, λ b, b ∧ c.eval α) tt
+  f.foldr (λ c, λ b, b && (c.eval α)) tt
+
+@[simp] theorem eval_nil {α : assignment} : eval α [] = tt := rfl
+
+@[simp] theorem eval_singleton {α : assignment} {c : clause} : eval α [c] = clause.eval α c := by simp [eval]
+
+theorem eval_cons {α : assignment} {c : clause} {f : cnf} : eval α (c :: f) = (clause.eval α c && eval α f) :=
+  by simp [eval, bool.band_comm]
+
+theorem eval_erase_of_mem {α : assignment} {c : clause} {f : cnf} (h : c ∈ f) : eval α f = (clause.eval α c) && (eval α (f.erase c)) :=
+begin
+  /-
+    induction c with d ds ih,
+  { exact absurd h (not_mem_nil _) },
+  rcases classical.em (l = d) with rfl | hne,
+  { simp [erase_cons_head, eval_cons] },
+  { simp only [eval_cons, erase_cons_tail ds (ne.symm hne), ih (mem_of_ne_of_mem hne h), ← bool.bor_assoc, bool.bor_comm] }
+  -/
+
+  induction f with cl cls ih,
+  { exact absurd h (not_mem_nil _) },
+  cases classical.em (c ~ cl),
+  sorry, sorry,
+end 
+
+/-! ### Counting -/
 
 /- Counts the number of clauses which evaluate to true under some assignment -/
 def count_tt (α : assignment) (f : cnf) : nat :=
-  list.length $ f.filter (λ c, c.eval α = tt)
+  length $ f.filter (λ c, c.eval α = tt)
 
 /- Counts the number of clauses which evaluate to false under some assignment -/
 def count_ff (α : assignment) (f : cnf) : nat :=
-  list.length $ f.filter (λ c, c.eval α = ff)
-
-/- Some useful simplifying statements -/
-lemma empty_eval_ff (α : assignment) (f : cnf) : f.length = 0 → f.eval α = tt :=
-begin
-  intro h,
-  rw list.length_eq_zero at h,
-  rw h,
-  unfold eval,
-  simp,
-end
-
--- Note: These proofs are identical to the ones above: simpler proof?
-lemma single_eval_clause [inhabited clause] (α : assignment) (f : cnf) : f.length = 1 → eval α f = f.head.eval α :=
-begin
-  intro h,
-  rw list.length_eq_one at h,
-  cases h with a ha,
-  unfold eval,
-  simp [ha],
-end
+  length $ f.filter (λ c, c.eval α = ff)
 
 end cnf
 
@@ -154,122 +114,353 @@ end cnf
 namespace explode
 
 open literal
+open clause
+open list
 
 /- This should ideally take in a nodup list or a finset, but lists are easier to manipulate -/
 /- Also, should ideally return a nodup list or a finset, see above comment -/
-def expl (l : list nat) : list clause :=
+-- Here is a non-recursive definition of expl. Recursive is easier though...
+def explode_non_rec (l : list nat) : list clause :=
   l.foldr (λ n, λ ls, (ls.map (λ e, (Pos n) :: e)) ++ (ls.map (λ e, (Neg n) :: e))) [[]]
 
+@[simp] lemma explode_non_rec_nil : explode_non_rec [] = [[]] := rfl
+
+@[simp] lemma explode_non_rec_cons {n : nat} {ns : list nat} : 
+  explode_non_rec (n :: ns) = (explode_non_rec ns).map (λ e, (Pos n) :: e) ++ (explode_non_rec ns).map (λ e, (Neg n) :: e) :=
+    by simp [explode_non_rec]
+
 /- Note: The nil case differs between the two. See if can fix above... -/
-def expl_rec : list nat → list clause 
-  | []        := []
-  | (n :: ns) :=
-  let
-    res := expl_rec ns
-  in
-    res.map (λ e, (Pos n) :: e) ++ res.map (λ e, (Neg n) :: e)
+def explode : list nat → list clause 
+  | []        := [[]]
+  | (n :: ns) := (explode ns).map (cons (Pos n)) ++ (explode ns).map (cons (Neg n))
 
-/- True if clause has even number of negated clauses, false otherwise -/
-def expl_parity (l : list nat) : list (clause × bool) :=
-  l.foldr (λ n, λ r,
-    (r.map (λ e, let (cl, par) := e in ⟨(Pos n) :: cl, par⟩) ++ 
-    (r.map (λ e, let (cl, par) := e in ⟨(Neg n) :: cl, bnot par⟩)))) [([], tt)]
-
-/- Counts the number of negated literals in each clause -/
-def expl_count (l : list nat) : list (clause × nat) :=
-  l.foldr (λ n, λ r,
-    (r.map (λ e, let (cl, c) := e in ⟨(Pos n) :: cl, c⟩) ++ 
-    (r.map (λ e, let (cl, c) := e in ⟨(Neg n) :: cl, c + 1⟩)))) [([], 0)]
-
--- Again, this proof is exactly the same as the eval single above
-lemma explode_single (l : list nat) : l.length = 1 → expl l = [[Pos l.head], [Neg l.head]] :=
+-- Saying they're equal is a little dangerous - maybe saying they're similar is good enough?
+theorem explode_and_explode_rec_equiv {ns : list nat} : explode_non_rec ns = explode ns :=
 begin
+  induction ns with m ms ih,
+  { simp [explode] },
+  { simp [explode, ih] }
+end
+
+theorem length_explode : ∀ (ns : list nat), length (explode ns) = 2^(length ns)
+| []        := rfl
+| (n :: ns) := by {
+  unfold explode,
+  unfold length,
+  rw pow_succ,
+  rw two_mul,
+  rw length_append,
+  repeat {rw length_map},
+  rw length_explode ns,
+}
+-- by simp [explode, length_explode ns, pow_succ, two_mul]
+-- was getting replace and stack space errors, so wrote out long-hand
+
+-- Corollary of the above theorem
+-- Can probably be reduced in length
+theorem length_explode_pos {ns : list nat} : length (explode ns) > 0 :=
+begin
+  rw length_explode ns,
+  induction ns with d hd,
+  { unfold length, simp },
+  { unfold length,
+    rw pow_succ,
+    rw two_mul,
+    exact add_pos (ns_ih) (ns_ih)}
+end
+
+-- Another corollary - is this needed?
+theorem exists_mem_of_explode : ∀ (ns : list nat), ∃ (c : clause), c ∈ explode ns :=
+  λ _, exists_mem_of_length_pos length_explode_pos
+
+theorem length_clause_explode {ns : list nat} : ∀ (c : clause), c ∈ explode ns → length c = length ns :=
+begin
+  induction ns with m ms ih,
+  { intros c h, unfold explode at h, rw (mem_singleton.mp h), refl},
+  simp only [explode, mem_cons_iff, mem_append, map_cons, mem_map],
+  rintros c (⟨c, hc, rfl⟩ | ⟨c, hc, rfl⟩);
+  { unfold length, rw ih c hc}
+end
+
+theorem mem_explode_of_mem {ns : list nat} : ∀ n ∈ ns, ∀ c ∈ explode ns, Pos n ∈ c ∨ Neg n ∈ c :=
+begin
+  induction ns with m ms ih,
+  { intros m hm, exact absurd hm (not_mem_nil _) },
+  simp only [explode, mem_cons_iff, mem_append, map_cons, mem_map],
+  rintros n (rfl | hn) c (⟨d, hd, rfl⟩ | ⟨d, hd, rfl⟩),
+  { left, apply mem_cons_self },
+  { right, apply mem_cons_self },
+  { cases ih n hn d hd with h h,
+    { left, apply mem_cons_of_mem _ h},
+    right, apply mem_cons_of_mem _ h},
+  { cases ih n hn d hd with h h,
+    { left, apply mem_cons_of_mem _ h},
+    right, apply mem_cons_of_mem _ h},
+end
+
+theorem not_mem_explode_of_not_mem {ns : list nat} : ∀ n ∉ ns, ∀ c ∈ explode ns, Pos n ∉ c ∧ Neg n ∉ c :=
+begin
+  induction ns with m ms ih,
+  { rintros m hm c hc,
+    simp [explode, hc] at hc,
+    simp [hc]},
+  simp only [explode, mem_append, map_cons, mem_map],
+  rintros p hp d hd,
+  rcases hd with ⟨c, ⟨hce, rfl⟩⟩ | ⟨c, ⟨hce, rfl⟩⟩,
+  rcases ih p (not_mem_of_not_mem_cons hp) c hce with ⟨hpos, hneg⟩,
+  { split,
+    { exact not_mem_cons_of_ne_of_not_mem (ne_pos_of_ne_nat (ne_of_not_mem_cons hp)) hpos},
+    exact not_mem_cons_of_ne_of_not_mem ne_lit_of_nat.symm hneg},
+  rcases ih p (not_mem_of_not_mem_cons hp) c hce with ⟨hpos, hneg⟩,
+  split,
+  exact not_mem_cons_of_ne_of_not_mem ne_lit_of_nat hpos,
+  exact not_mem_cons_of_ne_of_not_mem (ne_neg_of_ne_nat (ne_of_not_mem_cons hp)) hneg,
+end
+
+theorem mem_of_mem_explode {ns : list nat} : ∀ c ∈ explode ns, ∀ l ∈ c, literal.var l ∈ ns :=
+begin
+  induction ns with m ms ih,
+  { rintros c hc l hl,
+    simp [explode] at hc,
+    rw hc at hl,
+    exact absurd hl (not_mem_nil _)},
+  simp only [explode, mem_cons_iff, mem_append, map_cons, mem_map],
+  rintros c haor l hl,
+  rcases haor with ⟨a, ⟨hams, rfl⟩⟩ | ⟨a, ⟨hams, rfl⟩⟩,
+  { rcases hl with ⟨rfl, hla⟩,
+    { left, unfold var },
+    right, exact ih a hams l hl},
+  rcases hl with ⟨rfl | hlcons⟩,
+  { left, unfold var},
+  right, exact ih a hams l hl,
+end
+
+-- Another way to express this is to say for all literals where it and its opposite are not in c
+theorem not_mem_of_not_mem_explode {ns : list nat} : 
+  ∀ c ∈ explode ns, ∀ (n : nat), ((Pos n ∉ c) ∧ (Neg n ∉ c)) → n ∉ ns :=
+begin
+  induction ns with m ms ih,
+  { rintros _ _ _ _, exact not_mem_nil _},
+  simp only [explode, mem_append, map_cons, mem_map],
+  rintros c (⟨a, ⟨hams, rfl⟩⟩ | ⟨a, ⟨hams, rfl⟩⟩) n ⟨hpos, hneg⟩,
+
+  apply not_mem_cons_of_ne_of_not_mem,
+  { exact ne_nat_of_ne_pos (ne_of_not_mem_cons hpos) },
+  exact ih a hams n (and.intro (not_mem_of_not_mem_cons hpos) (not_mem_of_not_mem_cons hneg)),
+
+  apply not_mem_cons_of_ne_of_not_mem,
+  { exact ne_nat_of_ne_neg (ne_of_not_mem_cons hneg) },
+  exact ih a hams n (and.intro (not_mem_of_not_mem_cons hpos) (not_mem_of_not_mem_cons hneg)),
+end
+
+theorem xor_lit_of_explode_of_nodup_list {ns : list nat} (hnodup : list.nodup ns) : ∀ n ∈ ns, ∀ c ∈ explode ns, Pos n ∉ c ∨ Neg n ∉ c :=
+begin
+  induction ns with m ms ih,
+  { rintros _ hnil _ _, exact absurd hnil (not_mem_nil n)},
+  simp only [explode, mem_append, map_cons, mem_map],
+  rintros n hn c (⟨a, ⟨hams, rfl⟩⟩ | ⟨a, ⟨hams, rfl⟩⟩),
+  { rcases eq_or_ne_mem_of_mem hn with ⟨rfl | ⟨hn1, hn2⟩⟩, -- Why do hn1 and hn2 not appear?
+    { right, apply not_mem_cons_of_ne_of_not_mem, 
+      { exact ne_lit_of_nat.symm },
+      exact (not_mem_explode_of_not_mem m (nodup_cons.mp hnodup).left a hams).right },
+    cases h with h1 h2,
+    have ihred := ih ((nodup_cons.mp hnodup).right) n h2 a hams,
+    cases ihred,
+    { left, exact not_mem_cons_of_ne_of_not_mem (ne_pos_of_ne_nat h1) ihred},
+    right, exact not_mem_cons_of_ne_of_not_mem (ne_lit_of_nat.symm) ihred},
+  { rcases eq_or_ne_mem_of_mem hn with ⟨rfl | ⟨hn1, hn2⟩⟩,
+    { left, apply not_mem_cons_of_ne_of_not_mem,
+      { exact ne_lit_of_nat },
+      exact (not_mem_explode_of_not_mem m(nodup_cons.mp hnodup).left a hams).left },
+    cases h with h1 h2,
+    have ihred := ih ((nodup_cons.mp hnodup).right) n h2 a hams,
+    cases ihred,
+    { left, exact not_mem_cons_of_ne_of_not_mem ne_lit_of_nat ihred},
+    right, exact not_mem_cons_of_ne_of_not_mem (ne_neg_of_ne_nat h1) ihred}
+end
+
+/-
+theorem aaa {ns : list nat} (hnodup : list.nodup ns) : ∀ (c : clause), ∀ n ∈ ns, xor (Pos n ∈ c) (Neg n ∈ c) → ∃ e ∈ explode ns, c.equiv e :=
+begin
+  induction ns with m ms ih,
+  { rintros _ _ hnil _, exact absurd hnil (not_mem_nil n)},
+  rintros c n hn (⟨hpos, hnneg⟩ | ⟨hneg, hnnpos⟩),
+  { cases classical.em (n = m),
+    { have : m ∉ ms, from not_mem_of_nodup_cons hnodup, 
+      rw ← h at this,
+      have exi : ∃ (cl : clause), cl ∈ explode ms, from exists_mem_of_explode ms,
+      cases exi with cl clh,
+      use (Pos n) :: cl,
+      rw h,
+      unfold explode,
+      simp,
+      split,
+      {left, use cl, exact and.intro clh rfl},
+      sorry,
+    } sorry, sorry,}
+end
+
+theorem bbb {ns : list nat} (hnodup : list.nodup ns) : ∀ (c : clause), c.length = ns.length → (∀ n ∈ ns, xor (Pos n ∈ c) (Neg n ∈ c)) → ∃ e ∈ explode ns, c.equiv e :=
+begin
+  induction ns with m ms ih,
+  { intros c h _, 
+    use ([] : clause),
+    simp [explode, length_eq_zero.mp h]},
+  { rintros c hcl hn,
+    unfold length at hcl,
+    have msnodup : ms.nodup, from nodup_of_nodup_cons hnodup,
+    have sss := hn m (mem_cons_self m ms),
+    rcases sss with ⟨hpos, hnneg⟩ | ⟨hneg, hnpos⟩,
+    have len_erase : length (c.erase (Pos m)) = length c - 1, from length_erase_of_mem hpos,
+    have : length c - 1 = (length ms + nat.succ(0)) - 1, from congr_arg nat.pred hcl,
+    rw nat.add_succ_sub_one at this,
+    rw nat.add_zero at this,
+    rw ← len_erase at this,
+    have ihred := ih msnodup (c.erase (Pos m)) this,
+    have : ∀ (n : ℕ), n ∈ ms → xor (Pos n ∈ c.erase (Pos m)) (Neg n ∈ c.erase (Pos m)),
+      { intros n hnms, have : n ∈ (m :: ms), from mem_cons_of_mem m hnms,
+        have abcd := hn n this,
+        have erasems : (m :: ms).erase m = ms, from erase_cons_head m ms,
+        rw ← erasems at hnms,
+        have nm : n ≠ m, from ((mem_erase_iff_of_nodup hnodup).mp hnms).left,
+        sorry,
+      },
+    have := ihred this,
+    cases this with e he,
+    cases he with hhe hequiv,
+    use (Pos m :: e),
+    split,
+    { unfold explode,
+      simp,
+      use e,
+      exact and.intro hhe rfl },
+    { }
+  }
+end
+-/
+
+theorem perm_explode_of_perm {ns : list nat} : ∀ (l : list nat), l ~ ns → ∀ cn ∈ explode ns, ∃ cl ∈ explode l, cn ~ cl :=
+begin
+  induction ns with m ms ih,
+  { intro l, intro sim, intro cn, intro cn_sim, have : l = [], from perm.eq_nil sim, rw this,
+    unfold explode at cn_sim, have : cn = nil, from mem_singleton.mp cn_sim,
+    use ([] : clause),
+    unfold explode,
+    rw this,
+    exact and.intro (mem_singleton_self _) (perm.refl _)
+  },
+  {
+    intros l hlsim cn hcnexpl,
+    unfold explode at hcnexpl,
+    simp at hcnexpl,
+    cases hcnexpl,
+    have hlerase : l.erase m ~ (m :: ms).erase m, from perm.erase m hlsim,
+    have : (m :: ms).erase m = ms, from erase_cons_head m ms,
+    rw this at hlerase,
+    { cases hcnexpl with a ha, cases ha with ha1 ha2,
+      have ihred := ih (l.erase m) hlerase a ha1,
+      cases ihred with b hb,
+      cases hb with hb absim,
+      use (Pos m :: b),
+      sorry,
+     }, sorry,
+  }
+end
+
+-- The symbol '~' means a permutation between two lists, of which clauses are, under the hood
+theorem ccc {ns : list nat} (hnodup : list.nodup ns) : ∀ (c : clause), c.length = ns.length → (∀ n ∈ ns, xor (Pos n ∈ c) (Neg n ∈ c)) → ∃ e ∈ explode ns, c ~ e :=
+begin
+  sorry,
+end
+
+theorem ddd {ns : list nat} {n : nat} : ∀ c ∈ explode (n :: ns), ∃ cn ∈ explode ns, (Pos n :: cn) ~ c ∨ (Neg n :: cn) ~ c :=
+begin
+  induction ns with m ms ih,
+  { intros c hc, use nil, unfold explode at hc, simp at hc, split, simp [explode],
+    cases hc with hcp hcn, simp [hcp], simp [hcn]},
+  simp only [explode, mem_cons_iff, mem_append, map_cons, mem_map],
+  intro c,
   intro h,
-  rw list.length_eq_one at h,
-  cases h with a ha,
-  unfold expl,
-  simp [ha],
+  cases h with h1 h2, -- h is an or
+  cases h1 with a ha, -- h1 is and exists hyp
+  cases ha with ha1 ha2,
+  cases ha1 with ha1 ha1,
+  cases ha1 with a1 ha1,
+  cases ha1 with haa1 haa2,
+  sorry,
+  sorry,
+  sorry,
 end
 
-lemma explode_all_same_length (l : list nat) (len : l.length > 0) : ∀ c ∈ expl l, list.length c = list.length l :=
+theorem sim_erase_cons_of_explode {ns : list nat} {n : nat} (h : n ∈ ns) : ∀ c ∈ explode ns, ∃ cn ∈ explode (ns.erase n), (Pos n :: cn) ~ c ∨ (Neg n :: cn) ~ c :=
 begin
-  intros c h,
-  induction l,
-
-  -- This can probably be cleaned up
-  exfalso,
-  have : ([] : list nat) = [], from rfl,
-  have z : list.length [] = 0, from list.length_eq_zero.2 this,
-  rw z at len,
-  simp at len,
-  exact len,
-
-  -- Inudction hypothesis
-  cases l_tl,
-  have hd_len : [l_hd].length = 1, from list.length_singleton l_hd,
-  unfold expl at h,
-  simp at h,
-  cases h with hl hr,
-  rw hd_len,
-  simp [hl],
-
-  rw hd_len,
-  simp [hr],
-
-  have not_nil : (l_tl_hd :: l_tl_tl) ≠ list.nil, from list.cons_ne_nil l_tl_hd l_tl_tl,
-  have pos_len : (l_tl_hd :: l_tl_tl).length > 0, from list.length_pos_of_ne_nil not_nil,
-  have k := l_ih pos_len,
-  
-
-
+  induction ns with m ms ih,
+  { exact absurd h (not_mem_nil _) },
+  simp only [explode, mem_cons_iff, mem_append, map_cons, mem_map],
+  intros c hc,
+  cases hc with hcp hcn,
+  { cases hcp with a ha,
+    cases ha with ha1 ha2,
+    cases classical.em (n = m),
+    { use a, simp [h_1, erase_cons_head, ha2, ha1, perm.refl] },
+    { have ihred := ih (mem_of_ne_of_mem h_1 h) a ha1,
+      cases ihred with cn hcn,
+      cases hcn with hhcn hhhcn,
+      rw erase_cons_tail ms (ne.symm h_1),
+      rw ← ha2,
+      cases hhhcn,
+      { use (Pos m :: cn), unfold explode, split,
+        { simp only [mem_cons_iff, mem_append, map_cons, mem_map],
+          left, use cn, exact and.intro hhcn (and.intro (refl _) (refl _)) },
+        left, exact perm.trans (perm.swap (Pos m) (Pos n) cn) ((perm_cons (Pos m)).mpr hhhcn) },
+      { use (Pos m :: cn), unfold explode, split,
+        { simp only [mem_cons_iff, mem_append, map_cons, mem_map],
+          left, use cn, exact and.intro hhcn (and.intro (refl _) (refl _)) },
+        right, exact perm.trans (perm.swap (Pos m) (Neg n) cn) ((perm_cons (Pos m)).mpr hhhcn) }
+    }},
+  { cases hcn with a ha,
+    cases ha with ha1 ha2,
+    cases classical.em (n = m),
+    { use a, simp [h_1, erase_cons_head, ha2, ha1, perm.refl] },
+    { have ihred := ih (mem_of_ne_of_mem h_1 h) a ha1,
+      cases ihred with cn hcn,
+      cases hcn with hhcn hhhcn,
+      rw erase_cons_tail ms (ne.symm h_1),
+      rw ← ha2,
+      cases hhhcn,
+      { use (Neg m :: cn), unfold explode, split,
+        { simp only [mem_cons_iff, mem_append, map_cons, mem_map],
+          right, use cn, exact and.intro hhcn (and.intro (refl _) (refl _)) },
+        left, exact perm.trans (perm.swap (Neg m) (Pos n) cn) ((perm_cons (Neg m)).mpr hhhcn) },
+      { use (Neg m :: cn), unfold explode, split,
+        { simp only [mem_cons_iff, mem_append, map_cons, mem_map],
+          right, use cn, exact and.intro hhcn (and.intro (refl _) (refl _)) },
+        right, exact perm.trans (perm.swap (Neg m) (Neg n) cn) ((perm_cons (Neg m)).mpr hhhcn) } } }
 end
 
-lemma explode_count_accurate (l : list nat) (cl : clause) (c : nat) : ∀ e ∈ expl_count l, e = (cl, c) → clause.count_neg cl = c :=
+theorem explode_clause_perm_of_list {ns : list nat} : ∀ (c : clause), c ∈ explode ns → c.map var ~ ns :=
+begin 
+  induction ns with m ms ih,
+  { intros c hc, unfold explode at hc, rw (mem_singleton.mp hc), simp },
+  simp only [explode, mem_cons_iff, mem_append, map_cons, mem_map],
+  rintros c (⟨c, hc, rfl⟩ | ⟨c, hc, rfl⟩) ;
+  { simp [map, var, perm.cons m, ih c hc] }
+end
+
+--theorem explode_clause_cons_perm_of_list_cons {n : nat} {ns : list nat} :
+
+theorem backward {ns : list nat} : ∀ (c : clause), c.map var ~ ns → ∃ cl ∈ explode ns, c ~ cl :=
 begin
-  intros e h eq,
-  induction l,
-  unfold expl_count at h,
-  simp at h,
-  rw eq at h,
-  have k := prod.mk.inj h,
-  cases k with k1 k2,
-  rw k1,
-  unfold clause.count_neg,
-  simp,
-  symmetry,
-  exact k2,
-
-  -- Induction step
-  unfold expl_count at h,
-  simp at h,
-  cases h with hl hr,
-  
-end
-
---lemma exists_sat (l : list nat) (α : assignment) : l.length > 0 → ∃c ∈ expl l, clause.eval α c = tt :=
---begin
---  intro h,
---  induction l with n hn,
---  exfalso,
---  simp at h,
---  exact h,
-
-  -- Induction case
---  cases α n with hf ht,
---  sorry,
---  sorry,
---end
-
--- Cannot write clause for list literal here, for some reason
-/- States that for exploded var lists, any clause is a member -/
-/- This seems an overly complex definition... sets would be so much easier -/
---lemma all_mem_explode {ns : list nat} {c : list literal} (nsl : ns.length > 0) (cs_eq_c : c.length = ns.length) 
---  : (∀i, (0 ≤ i ∧ i < c.length) ∧ ∃ (cl : literal), list.nth c i = some cl ∧ ∃ (nn : nat), list.nth ns i = some nn ∧ cl.var = nn) → c ∈ expl ns :=
---∀ l ∈ c, literal.var l ∈ ns) → c ∈ expl ns :=
---begin
---  intro i,
---  intro h,
-
---end
+  induction ns with m ms ih,
+  { simp [explode, perm_nil] },
+  rintros c h,
+  have : (map var c).erase m ~ (m :: ms).erase m, from perm.erase m h,
+  rw erase_cons_head m at this,
+  have hm : m ∈ map var c, from h.mem_iff.mpr (mem_cons_self m ms),
+  have : ∃ l, l ∈ c ∧ var l = m, from mem_map.mp hm,
+  cases this with l hl,
+  cases hl with hl1 hl2,
+  sorry, 
+end 
 
 end explode
