src/cnf/clause.lean
@@ -1,0 +1,104 @@
+/-
+This file contains the definition of a Boolean (disjunctive) clause (as in CNF).
+This particular implementation has clauses as lists.
+
+Authors: Cayden Codel, Jeremy Avigad, Marijn Heule
+Carnegie Mellon Univeristy
+-/
+
+import cnf.literal
+import basic
+import data.list.basic
+import data.list.perm
+
+/- (Disjunctive) clauses are lists of literals, joined by logical ORs. -/
+def clause := list literal
+
+namespace clause
+
+open literal
+open list
+
+instance : inhabited clause := ⟨[default literal]⟩
+
+instance has_decidable_eq [s : decidable_eq literal] : decidable_eq clause
+| []        []        := is_true rfl
+| (a :: as) []        := is_false (λ h, list.no_confusion h)
+| []        (b :: bs) := is_false (λ h, list.no_confusion h)
+| (a :: as) (b :: bs) :=
+  match s a b with
+  | is_true hab  :=
+    match has_decidable_eq as bs with
+    | is_true habs  := is_true (eq.subst hab (eq.subst habs rfl))
+    | is_false nabs := is_false (λ h, list.no_confusion h (λ _ habs, absurd habs nabs))
+    end
+  | is_false nab := is_false (λ h, list.no_confusion h (λ hab _, absurd hab nab))
+  end
+
+instance : has_mem literal clause := ⟨list.mem⟩
+
+instance : has_emptyc clause := ⟨list.nil⟩
+
+instance : has_union clause := ⟨list.union⟩
+
+instance : has_inter clause := ⟨list.inter⟩
+
+instance : has_singleton literal clause := ⟨λ l, [l]⟩ 
+
+instance : has_insert literal clause := ⟨list.insert⟩
+
+instance : has_append clause := ⟨list.append⟩
+
+/- The clause represents a disjunction, so we evaluate literals until tt is found -/
+def eval (α : assignment) (c : clause) : bool :=
+  c.foldr (λ l b, b || (l.eval α)) ff
+
+@[simp] theorem eval_nil {α : assignment} : eval α [] = ff := rfl
+
+@[simp] theorem eval_singleton {α : assignment} {l : literal} : eval α [l] = literal.eval α l := by simp [eval]
+
+theorem eval_cons {α : assignment} {l : literal} {c : clause} : eval α (l :: c) = (literal.eval α l) || (eval α c) :=
+  by simp [eval, bool.bor_comm]
+
+theorem eval_erase_of_mem {α : assignment} {l : literal} {c : clause} (h : l ∈ c) : eval α c = (literal.eval α l) || (eval α (c.erase l)) :=
+begin
+  induction c with d ds ih,
+  { exact absurd h (not_mem_nil _) },
+  rcases classical.em (l = d) with rfl | hne,
+  { simp [erase_cons_head, eval_cons] },
+  { simp only [eval_cons, erase_cons_tail ds (ne.symm hne), ih (mem_of_ne_of_mem hne h), ← bool.bor_assoc, bool.bor_comm] }
+end
+
+theorem eval_erase_of_not_mem {α : assignment} {l : literal} {c : clause} (h : l ∉ c) : eval α c = eval α (c.erase l) :=
+  by simp [erase_of_not_mem h]
+
+/-! ### Similarity of clauses -/
+-- Because clauses are literals joined by ORs, and OR is commutative, similar clauses evaluate identically
+
+theorem eval_sim {α : assignment} {c₁ : clause} : ∀ (c₂ : clause), c₁ ~ c₂ → eval α c₁ = eval α c₂ :=
+begin
+  induction c₁ with l c ih; intros c₂ h,
+  { simp [perm.nil_eq h] },
+  { simp only [ih (c₂.erase l) (cons_perm_iff_perm_erase.mp h).2, 
+      eval_cons, (eval_erase_of_mem ((perm.mem_iff h).mp (mem_cons_self l c))).symm] }
+end
+
+
+/-! ### Counting -/
+/- Counts the number of literals that evaluate to true in the clause, under some assignment -/
+def count_tt (α : assignment) (c : clause) : nat :=
+  length $ c.filter (λ l, l.eval α = tt)
+
+/- Counts the number of literals that evaluate to false in the clause, under some assignment -/
+def count_ff (α : assignment) (c : clause) : nat :=
+  length $ c.filter (λ l, l.eval α = ff)
+
+/- Counts the number of positive literals in the clause -/
+def count_pos (c : clause) : nat :=
+  length $ c.filter (λ l, l.is_pos)
+
+/- Counts the number of negative literals in the clause -/
+def count_neg (c : clause) : nat :=
+  length $ c.filter (λ l, literal.is_neg l)
+
+end clause
