src/cnf/clause_set.lean
@@ -1,0 +1,90 @@
+/-
+
+  This file contains the definition of a Boolean (disjunctive) clause (as in CNF).
+  This particular implementation has clauses as finsets.
+
+  Authors: Cayden Codel, Jeremy Avigad, Marijn Heule
+  Carnegie Mellon Univeristy
+
+-/
+
+import data.finset
+import cnf.literal
+import basic
+
+/- 
+  (Disjunctive) clauses are finite sets of literals.
+  The finite set represents the literals joined by logical ORs.
+-/
+def clause := finset literal
+
+namespace clause
+
+instance : has_mem literal clause := ⟨λ l c, l ∈ c.1⟩
+
+-- TODO why is the mem_def and has_mem theorems/instance features required?
+theorem mem_def {l : literal} {c : clause} : l ∈ c ↔ l ∈ c.1 := iff.rfl
+
+instance : has_emptyc (clause) := ⟨finset.empty⟩
+
+-- Define some equality
+--instance has_decidable_eq : decidable_eq clause := sorry
+
+instance : has_union (clause) := ⟨λ c₁ c₂, ⟨_, multiset.nodup_ndunion c₁.1 c₂.2⟩⟩
+
+instance : has_singleton literal clause := ⟨λ l, ⟨{l}, list.nodup_singleton l⟩⟩ 
+
+instance : has_insert literal clause := ⟨λ l c, ⟨_, multiset.nodup_ndinsert l c.2⟩⟩
+
+theorem insert_def (l : literal) (c : clause) : insert l c = ⟨_, multiset.nodup_ndinsert l c.2⟩ := rfl
+
+def erase (c : clause) (l : literal) : clause := ⟨_, multiset.nodup_erase_of_nodup l c.2⟩
+
+/- The clause represents a disjunction, so we evaluate literals until tt is found -/
+def eval (α : assignment) (c : clause) : bool :=
+  cond (c.card > 0) (cond (∃ l ∈ c, literal.eval α l = tt) tt ff) ff
+
+/- Counts the number of literals that evaluate to true in the clause, under some assignment -/
+def count_tt (α : assignment) (c : clause) : nat :=
+  finset.card $ c.filter (λ l, l.eval α = tt)
+
+/- Counts the number of literals that evaluate to false in the clause, under some assignment -/
+def count_ff (α : assignment) (c : clause) : nat :=
+  finset.card $ c.filter (λ l, l.eval α = ff)
+
+/- Counts the number of positive literals in the clause -/
+/- TODO why can't I use a match statement? Requires decidable_pred... -/
+def count_pos (c : clause) : nat :=
+  --list.length $ c.filter (λ l, match l with | (literal.Pos _) := true | _ := false end)
+  finset.card $ c.filter (λ l, literal.is_pos l = tt)
+
+/- Counts the number of negative literals in the clause -/
+def count_neg (c : clause) : nat :=
+  finset.card $ c.filter (λ l, literal.is_neg l = tt)
+
+/- Some useful statements for proofs of clauses -/
+lemma empty_eval_ff {α : assignment} {c : clause} : c.card = 0 → eval α c = ff :=
+begin
+  -- This proof is very similar to the one for lists (change card to length)
+  intro h,
+  rw finset.card_eq_zero at h,
+  rw h,
+  unfold eval,
+  simp,
+end
+
+-- TODO not sure whether to have this be forall or exists...
+lemma single_eval_lit [inhabited literal] {α : assignment} {c : clause} : c.card = 1 → ∀ l ∈ c, eval α c = literal.eval α l :=
+begin
+  intros h l hin,
+  rw finset.card_eq_one at h,
+  cases h with a ha,
+  rw ha at hin,
+  have : l = a, from finset.mem_singleton.mp hin,
+  rw this,
+  rw ha,
+  unfold eval,
+  simp,
+end
+
+end clause
