src/cnf/literal.lean
@@ -1,0 +1,125 @@
+/-
+
+  This file contains the definition of a Boolean literal.#check
+  
+  Authors: Cayden Codel, Jeremy Avigad, Marijn Heule
+  Carnegie Mellon University
+
+-/
+
+import init.data.nat
+
+/- 
+  All propositional formulas are comprised of Boolean variables.
+  Here, we represent variables as natural numbers, which may then be evaluated
+  with an appropriate assignment of boolean values to those variables.
+
+  Literals are positive and negative instances of those variables.
+-/
+inductive literal : Type
+  | Pos : nat → literal
+  | Neg : nat → literal
+
+/- Assignments give boolean values to the variables -/
+def assignment := nat → bool
+
+namespace literal
+
+/- Instance properties -/
+instance : inhabited literal := ⟨Pos 0⟩
+
+instance has_decidable_eq : decidable_eq literal
+  | (Pos n) (Pos m) :=
+    match nat.decidable_eq n m with
+      | is_true hnm   := is_true (hnm ▸ eq.refl (Pos n))
+      | is_false hneq := is_false (λ h, literal.no_confusion h (λ habs, absurd habs hneq))
+    end
+  | (Pos _) (Neg _) := is_false (λ h, literal.no_confusion h)
+  | (Neg _) (Pos _) := is_false (λ h, literal.no_confusion h)
+  | (Neg n) (Neg m) :=
+    match nat.decidable_eq n m with
+      | is_true hnm   := is_true (hnm ▸ eq.refl (Neg n))
+      | is_false hneq := is_false (λ h, literal.no_confusion h (λ habs, absurd habs hneq))
+    end
+
+/- Extracts the natural number boolean variable of the literal -/
+def var : literal → nat
+  | (Pos n) := n
+  | (Neg n) := n
+
+/- Negated literals receive the opposite boolean value as the variable -/
+def eval (α : assignment) : literal → bool
+  | (Pos n) := α n
+  | (Neg n) := bnot (α n)
+
+/- Flips the parity of the literal from positive to negative and vice versa -/
+def flip : literal → literal
+  | (Pos n) := Neg n
+  | (Neg n) := Pos n
+
+lemma eval_flip {α : assignment} : ∀ (l : literal), eval α l = bnot (eval α l.flip)
+| (Pos n) := by simp [flip, eval]
+| (Neg n) := by simp [flip, eval]
+
+lemma eval_flip_flip {α : assignment} : ∀ (l : literal), eval α l = eval α l.flip.flip
+| (Pos n) := by simp [flip]
+| (Neg n) := by simp [flip]
+
+/- Sets the literal to the positive form -/
+def set_pos : literal → literal
+  | (Pos n) := Pos n
+  | (Neg n) := Pos n
+
+/- Sets the literal to the negative form -/
+def set_neg : literal → literal
+  | (Pos n) := Neg n
+  | (Neg n) := Neg n
+
+/- Returns tt if the literal is positive, ff otherwise -/
+def is_pos : literal → bool
+  | (Pos _) := tt
+  | (Neg _) := ff
+
+/- Returns tt if the literal is negative, ff otherwise -/
+def is_neg : literal → bool
+  | (Pos _) := ff
+  | (Neg _) := tt
+
+-- This seems like a lot of casing... can this be generalized?
+
+@[simp] lemma ne_pos_neg_of_nat {n : nat} : Pos n ≠ Neg n := dec_trivial
+
+@[simp] lemma ne_nat_of_ne_pos {n m : nat} (h : Pos n ≠ Pos m) : n ≠ m :=
+begin
+  intro heq,
+  exact absurd (congr_arg Pos heq) h,
+end
+
+@[simp] lemma ne_nat_of_ne_neg {n m : nat} (h : Neg n ≠ Neg m) : n ≠ m :=
+begin
+  intro heq,
+  exact absurd (congr_arg Neg heq) h,
+end
+
+@[simp] theorem ne_lit_of_ne_nat {n m : nat} (h : n ≠ m) : Pos n ≠ Neg m := dec_trivial
+
+@[simp] theorem ne_lit_of_nat {n m : nat} : Pos n ≠ Neg m :=
+begin
+  cases classical.em (n = m) with he hne,
+  { rw he, exact ne_pos_neg_of_nat},
+  exact ne_lit_of_ne_nat hne,
+end
+
+@[simp] theorem ne_pos_of_ne_nat {n m : nat} (h : n ≠ m) : Pos n ≠ Pos m :=
+begin
+  intro hp,
+  exact absurd (congr_arg var hp) h,
+end
+
+@[simp] theorem ne_neg_of_ne_nat {n m : nat} (h : n ≠ m) : Neg n ≠ Neg m :=
+begin
+  intro hp,
+  exact absurd (congr_arg var hp) h,
+end
+
+end literal
